theories/heap_lang/lib/membrane.v
@@ -84,17 +84,12 @@ Section proof.
 
   Notation lowval := (low : val → iProp Σ).
 
-  (*
-	PDS: The spec can be improved to properly track progress bits
-	rather than accept the least common denominator: Wrap (unwrap)
-	only gets stuck if locout (locin) does.
-  *)
-  Lemma wrap_unwrap :
-    is_monP locout Ψ low -∗
-    is_monP locin low Ψ -∗
-    □ ((∀ p E Φ, ▷(∀ v, is_monP v (on_val Ψ) lowval -∗ Φ v) -∗
+  Lemma wrap_unwrap p1 p2 :
+    is_monP p1 locout Ψ low -∗
+    is_monP p2 locin low Ψ -∗
+    □ ((∀ p E Φ, ▷(∀ v, is_monP p1 v (on_val Ψ) lowval -∗ Φ v) -∗
       WP membrane locout locin @ p; E {{ Φ }}) ∗
-     (∀ p E Φ, ▷(∀ v, is_monP v lowval (on_val Ψ) -∗ Φ v) -∗
+     (∀ p E Φ, ▷(∀ v, is_monP p2 v lowval (on_val Ψ) -∗ Φ v) -∗
       WP membrane locin locout @ p; E {{ Φ }}))%I.
   Proof.
     iIntros "#Hlocout #Hlocin".
@@ -104,7 +99,8 @@ Section proof.
     - iIntros (p E Φ) "HΦ". wp_rec. wp_lam.
       iApply "HΦ". clear Φ. iIntros (v) "!#". iIntros (Φ) "#Hv HΦ". wp_lam.
       wp_apply "IHmkw". iIntros (wrap) "#Hwrap". iClear "IHmkw".
-        rewrite (monP_triple wrap). setoid_rewrite always_elim. wp_let.
+        rewrite (monP_triple _ wrap). setoid_rewrite always_elim.
+        wp_let.
 
       (* Wrapping functions. *)
       wp_typecast Hrec.
@@ -113,19 +109,22 @@ Section proof.
         destruct (is_rec_val _ Hrec) as (f&x&erec&?&->).
           rewrite on_val_rec always_elim. wp_match.
         wp_apply "IHmku". iIntros (unwrap) "#Hunwrap". iClear "IHmku".
-          rewrite (monP_triple unwrap). wp_let.
+          rewrite (monP_triple _ unwrap).
+          setoid_rewrite (wp_forget_progress p2).
+          wp_let.
         iApply "HΦ". clear Φ.
         rewrite low_val. iAlways. iNext. iIntros (v1) "Hv1".
           simpl_subst.
         wp_apply ("Hunwrap" with "* Hv1"). iIntros (v2) "Hv2". wp_rec.
         wp_apply ("Hv" with "Hv2"). iIntros (v3) "Hv3".
+          setoid_rewrite (wp_forget_progress p1 _ (wrap _)).
         wp_apply ("Hwrap" with "* Hv3"). by iIntros.
       wp_match. iClear "IHmku Hlocin".
 
       (* Wrapping locations. *)
       wp_typecast Hloc; wp_match.
       + destruct (is_loc_val _ Hloc) as (l&->).
-          rewrite on_val_elim (monP_triple locout).
+          rewrite on_val_elim (monP_triple _ locout).
         wp_apply ("Hlocout" with "* Hv"). iIntros (v1) "Hv1".
         iApply "HΦ". by rewrite low_val.
       iClear "Hlocout".
@@ -173,7 +172,8 @@ Section proof.
     - iIntros (p E Φ) "HΦ". wp_rec. wp_lam.
       iApply "HΦ". clear Φ. iIntros (v) "!#". iIntros (Φ) "#Hv HΦ". wp_lam.
       wp_apply "IHmku". iIntros (unwrap) "#Hunwrap". iClear "IHmku".
-        rewrite (monP_triple unwrap). setoid_rewrite always_elim. wp_let.
+        rewrite (monP_triple _ unwrap). setoid_rewrite always_elim.
+        wp_let.
 
       (* Unwrapping functions. *)
       wp_typecast Hrec.
@@ -182,19 +182,22 @@ Section proof.
         destruct (is_rec_val v Hrec) as (f&x&erec&?&->).
           rewrite low_rec always_elim. wp_match.
         wp_apply "IHmkw". iIntros (wrap) "#Hwrap". iClear "IHmkw".
-          rewrite (monP_triple wrap). wp_let.
+          rewrite (monP_triple _ wrap).
+          setoid_rewrite (wp_forget_progress p1 _ (wrap _)).
+          wp_let.
         iApply "HΦ". clear Φ.
         rewrite on_val_elim. iAlways. iNext. iIntros (v1) "Hv1".
           simpl_subst.
         wp_apply ("Hwrap" with "* Hv1"). iIntros (v2) "Hv2". wp_rec.
         wp_apply ("Hv" with "Hv2"). iIntros (v3) "Hv3".
+          setoid_rewrite (wp_forget_progress p2 _ (unwrap _)).
         wp_apply ("Hunwrap" with "* Hv3"). by iIntros.
       wp_match. iClear "IHmkw Hlocout".
 
       (* Unwrapping locations. *)
       wp_typecast Hloc; wp_match.
       + destruct (is_loc_val _ Hloc) as (l1&->).
-          rewrite low_val (monP_triple locin).
+          rewrite low_val (monP_triple _ locin).
         wp_apply ("Hlocin" with "* Hv"). iIntros (l2) "Hl2".
         iApply "HΦ". rewrite on_val_elim. by iFrame.
       iClear "Hlocin".
@@ -245,20 +248,20 @@ Section proof.
 	locations to reference monitors (of type [on_val Ψ → low]) on
 	values.
   *)
-  Lemma membrane_wrap_spec p E :
-    {{{ is_monP locout Ψ low ∗ is_monP locin low Ψ }}}
+  Lemma membrane_wrap_spec p E p1 p2 :
+    {{{ is_monP p1 locout Ψ low ∗ is_monP p2 locin low Ψ }}}
       membrane locout locin @ p; E
-    {{{ wrap, RET wrap; is_monP wrap (on_val Ψ) lowval }}}.
+    {{{ wrap, RET wrap; is_monP p1 wrap (on_val Ψ) lowval }}}.
   Proof.
     iIntros (Φ) "[Hout Hin] HΦ".
     iDestruct (wrap_unwrap with "Hout Hin") as "(Hw & _)".
     by iApply "Hw".
   Qed.
 
-  Lemma membrane_unwrap_spec p E :
-    {{{ is_monP locout Ψ low ∗ is_monP locin low Ψ }}}
+  Lemma membrane_unwrap_spec p E p1 p2 :
+    {{{ is_monP p1 locout Ψ low ∗ is_monP p2 locin low Ψ }}}
       membrane locin locout @ p; E
-    {{{ unwrap, RET unwrap; is_monP unwrap lowval (on_val Ψ) }}}.
+    {{{ unwrap, RET unwrap; is_monP p2 unwrap lowval (on_val Ψ) }}}.
   Proof.
     iIntros (Φ) "[Hout Hin] HΦ".
     iDestruct (wrap_unwrap with "Hout Hin") as "(_ & Hu)".
@@ -292,24 +295,52 @@ Section inert.
   Implicit Types l : loc.
   Implicit Types v : val.
   Import notation.
+  Notation lowval := (low : val → iProp Σ).
 
   Definition inert : val → iProp Σ := on_val (const True%I).
-  Definition is_locout (locout : val) : iProp Σ :=
-    (∀ l1, {{{ True }}} locout l1 ?{{{ l2, RET LocV l2; low l2 }}})%I.
-  Definition is_locin (locin : val) : iProp Σ :=
-    (∀ l2, {{{ low l2 }}} locin l2 ?{{{ l1, RET LocV l1; True }}})%I.
-  Definition is_wrap (wrap : val) : iProp Σ :=
-    (∀ v1, {{{ inert v1 }}} wrap v1 ?{{{ v2, RET v2; low v2 }}})%I.
 
-  Lemma inert_membrane_spec p E locout locin :
-    {{{ is_locout locout ∗ is_locin locin }}}
+  Definition is_locout (p1 : pbit) (locout : val) : iProp Σ :=
+    is_monP p1 locout (const True%I) low.
+  Definition is_locin (p2 : pbit) (locin : val) : iProp Σ :=
+    is_monP p2 locin lowloc (const True%I).
+  Definition is_wrap (p1 : pbit) (wrap : val) : iProp Σ :=
+    is_monP p1 wrap inert lowval.
+  Definition is_unwrap (p2 : pbit) (unwrap : val) : iProp Σ :=
+    is_monP p2 unwrap lowval inert.
+
+  Lemma locout_triple p1 locout :
+    is_locout p1 locout ⊣⊢
+    (∀ l1, {{{ True }}} locout l1 @ p1; ⊤ {{{ l2, RET LocV l2; low l2 }}})%I.
+  Proof. by []. Qed.
+
+  Lemma locin_triple p2 locin :
+    is_locin p2 locin ⊣⊢
+    (∀ l2, {{{ low l2 }}} locin l2 @ p2; ⊤ {{{ l1, RET LocV l1; True }}})%I.
+  Proof. by []. Qed.
+
+  Lemma wrap_triple p1 wrap :
+    is_wrap p1 wrap ⊣⊢
+    (∀ v1, {{{ inert v1 }}} wrap v1 @ p1; ⊤ {{{ v2, RET v2; low v2 }}})%I.
+  Proof. by []. Qed.
+
+  Lemma unwrap_triple p2 unwrap :
+    is_unwrap p2 unwrap ⊣⊢
+    (∀ v2, {{{ low v2 }}} unwrap v2 @ p2; ⊤ {{{ v1, RET v1; inert v1 }}})%I.
+  Proof. by []. Qed.
+
+  Lemma inert_wrap_spec p E locout locin p1 p2 :
+    {{{ is_locout p1 locout ∗ is_locin p2 locin }}}
       membrane locout locin @ p; E
-    {{{ wrap, RET wrap; is_wrap wrap }}}.
+    {{{ wrap, RET wrap; is_wrap p1 wrap }}}.
   Proof.
-    iIntros (Φ) "#(Hout & Hin)". rewrite -membrane_wrap_spec. clear Φ. iSplit.
-    - iIntros (l) "!#". iIntros (Φ) "_ HΦ".
-      by iApply ("Hout" $! l with "[] HΦ").
-    - iIntros (l) "!#". iIntros (Φ) "Hl HΦ".
-      by iApply ("Hin" $! l with "Hl HΦ").
+    iIntros (Φ) "#(?&?)". rewrite -membrane_wrap_spec. by iSplit.
+  Qed.
+
+  Lemma inert_unwrap_spec p E locout locin p1 p2 :
+    {{{ is_locout p1 locout ∗ is_locin p2 locin }}}
+      membrane locin locout @ p; E
+    {{{ unwrap, RET unwrap; is_unwrap p2 unwrap }}}.
+  Proof.
+    iIntros (Φ) "#(?&?)". rewrite -membrane_unwrap_spec. by iSplit.
   Qed.
 End inert.
