theories/heap_lang/lib/monitor.v
@@ -1,6 +1,8 @@
 From iris.heap_lang Require Export heap.
 From iris.heap_lang.lib Require Export constructor.
 From iris.heap_lang Require notation.
+From iris.proofmode Require Import tactics.
+Import uPred.
 
 (* Minor annoyance: [solve_proper] can't handle our goals. *)
 Local Notation ext R := (pointwise_relation _ R).
@@ -17,39 +19,45 @@ Ltac solve_proper_eq :=
 
 (** * Reference monitors *)
 (**
-	The assertion [is_mon v Ψ1 Ψ2] means that [v] is a reference
-	monitor of "type" [Ψ1 → Ψ2] where [Ψ1] is a predicate on
-	inputs of type [A] and [Ψ2] relates inputs of type [A] to
-	outputs of type [B]. Both [A] and [B] must have [constructor]
-	instances.
+	The assertion [is_mon p v R Ψ1 Ψ2] means that [v] is a
+	reference monitor (with progress bit [p]) of "type" [Ψ1 → Ψ2]
+	where [Ψ1] is a predicate on inputs of type [A] and [Ψ2]
+	relates inputs of type [A] to outputs of type [B]. Both [A]
+	and [B] must have [constructor] instances.
 *)
 Section is_mon.
   Context `{heapG Σ, fA : constructor A, fB : constructor B}.
 
-  Definition is_mon (v : val) (Ψ1 : A → iProp Σ)
+  Definition is_mon (p : pbit) (v : val) (Ψ1 : A → iProp Σ)
       (Ψ2 : A → B → iProp Σ) : iProp Σ :=
-    (∀ a, {{{ Ψ1 a }}} v (fA a) ?{{{ b, RET fB b; Ψ2 a b }}})%I.
+    (∀ a, {{{ Ψ1 a }}} v (fA a) @ p; ⊤ {{{ b, RET fB b; Ψ2 a b }}})%I.
 
-  Global Instance is_mon_persistent v Ψ1 Ψ2 :
-    PersistentP (is_mon v Ψ1 Ψ2).
+  Global Instance is_mon_persistent p v Ψ1 Ψ2 :
+    PersistentP (is_mon p v Ψ1 Ψ2).
   Proof. apply _. Qed.
 
-  Global Instance is_mon_ne v n :
-    Proper (ext (dist n) ==> ((=) ==> ext (dist n)) ==> dist n) (is_mon v).
+  Global Instance is_mon_ne p v n :
+    Proper (ext (dist n) ==> ((=) ==> ext (dist n)) ==> dist n) (is_mon p v).
   Proof. solve_proper_eq. Qed.
 
-  Global Instance is_mon_proper v :
-     Proper (ext (≡) ==> ((=) ==> ext (≡)) ==> (≡)) (is_mon v).
+  Global Instance is_mon_proper p v :
+     Proper (ext (≡) ==> ((=) ==> ext (≡)) ==> (≡)) (is_mon p v).
   Proof. solve_proper_eq. Qed.
+
+  Lemma mon_triple p v Ψ1 Ψ2 :
+    is_mon p v Ψ1 Ψ2 ⊣⊢
+    (∀ a, {{{ Ψ1 a }}} v (fA a) @ p; ⊤ {{{ b, RET fB b; Ψ2 a b }}})%I.
+  Proof. by []. Qed.
 End is_mon.
 Typeclasses Opaque is_mon.
 
 (** * Predicate-based reference monitors *)
 (**
-	The assertion [is_monP v Ψ1 Ψ2] means that [v] is a reference
-	monitor of "type" [Ψ1 → Ψ2] where [Ψ1] and [Ψ2] are predicates
-	on inputs of type [A] and outputs of type [B], respectively.
-	Both [A] and [B] must have [constructor] instances.
+	The assertion [is_monP p v R Ψ1 Ψ2] means that [v] is a
+	reference monitor (with progress bit [p]) of "type" [Ψ1 → Ψ2]
+	where [Ψ1] and [Ψ2] are predicates on inputs of type [A] and
+	outputs of type [B], respectively. Both [A] and [B] must have
+	[constructor] instances.
 
 	This is just a special case of [is_mon] where [Ψ2] does not
 	depend on the input.
@@ -57,10 +65,11 @@ Typeclasses Opaque is_mon.
 Section is_monP.
   Context `{heapG Σ, fA : constructor A, fB : constructor B}.
 
-  Definition is_monP (v : val) (Ψ1 : A → iProp Σ)
-      (Ψ2 : B → iProp Σ) : iProp Σ := is_mon v Ψ1 (λ _, Ψ2).
+  Definition is_monP (p : pbit) (v : val) (Ψ1 : A → iProp Σ)
+      (Ψ2 : B → iProp Σ) : iProp Σ := is_mon p v Ψ1 (λ _, Ψ2).
 
-  Lemma monP_triple v Ψ1 Ψ2 :
-    is_monP v Ψ1 Ψ2 ⊣⊢ (∀ a, {{{ Ψ1 a }}} v (fA a) ?{{{ b, RET fB b; Ψ2 b }}})%I.
+  Lemma monP_triple p v Ψ1 Ψ2 :
+    is_monP p v Ψ1 Ψ2 ⊣⊢
+    (∀ a, {{{ Ψ1 a }}} v (fA a) @ p; ⊤ {{{ b, RET fB b; Ψ2 b }}})%I.
   Proof. by []. Qed.
 End is_monP.
